Is0/Lemmas.lean
@@ -13,11 +13,11 @@ section WithCirgen
 
 open CirgenNotation
 
-lemma Cirgen.step_Sequence_Assign_collapsible {state : State} {name : String} {op : Op} {program : Cirgen} :
+lemma Cirgen.run_Sequence_Assign_collapsible {state : State} {name : String} {op : Op} {program : Cirgen} :
     Γ state ⟦name ←ₐ op; program⟧ = Γ (state[name] := Γ state ⟦op⟧) ⟦program⟧ := by
-  cases op <;> conv => lhs; simp [Cirgen.step, State.update, Map.update, beq_iff_eq]
+  cases op <;> conv => lhs; simp [Cirgen.run, State.update, Map.update, beq_iff_eq]
 
-lemma Cirgen.step_Sequence_Set_collapsible
+lemma Cirgen.run_Sequence_Set_collapsible
     {state : State}
     {name : String}
     {nameₓ : String}
@@ -27,22 +27,22 @@ lemma Cirgen.step_Sequence_Set_collapsible
     (h : state.buffers name = some buffer)
     (h₁ : state.felts nameₓ = some x) :
     Γ state ⟦⟨name⟩[i] ←ₐ ⟨nameₓ⟩; program⟧ = 
-    Γ { state with buffers := state.buffers[name] := buffer.set i x } ⟦program⟧ := by simp [step, *]
+    Γ { state with buffers := state.buffers[name] := buffer.set i x } ⟦program⟧ := by simp [run, *]
 
-lemma Cirgen.step_if_true {c : Variable Felt}
+lemma Cirgen.run_if_true {c : Variable Felt}
   (h : st.felts c.name = some 0) :
   Γ st ⟦guard c then prog⟧ = (st, none) := by
-  simp only [step]; generalize eq : st.felts c.name = cond
+  simp only [run]; generalize eq : st.felts c.name = cond
   rcases cond with _ | ⟨x⟩ <;> simp only <;> rw [eq] at h
   · cases h
   · simp; exact λ contra => absurd (by injection h) contra
 
-lemma Cirgen.step_if_false {c : Variable Felt}
+lemma Cirgen.run_if_false {c : Variable Felt}
   (x : Felt)
   (h₁ : st.felts c.name = some x)
   (h₂ : x ≠ 0) :
   Γ st ⟦guard c then prog⟧ = Γ st ⟦prog⟧ := by
-  simp only [step]; generalize eq : st.felts c.name = cond
+  simp only [run]; generalize eq : st.felts c.name = cond
   rcases cond with _ | ⟨y⟩ <;> simp only <;> rw [eq] at h₁
   · cases h₁
   · simp; intros contra
@@ -50,13 +50,13 @@ lemma Cirgen.step_if_false {c : Variable Felt}
     injection h₁ with contra
     exact absurd contra.symm h₂
 
-lemma Cirgen.step_seq :
+lemma Cirgen.run_seq :
   Γ st ⟦p₁; p₂⟧ = let (st', x) := Γ st ⟦p₁⟧
                   match x with
                     | some x => (st', some x)
                     | none => Γ st' ⟦p₂⟧ := rfl
 
-lemma Cirgen.step_Sequence_If_collapsible
+lemma Cirgen.run_Sequence_If_collapsible
     {state : State}
     {name : String}
     {branch : Cirgen}
@@ -68,12 +68,12 @@ lemma Cirgen.step_Sequence_If_collapsible
       then Γ state ⟦program⟧
       else Γ state ⟦branch; program⟧ := by
     generalize eq : (x == 0) = cond
-    rw [step_seq]
+    rw [run_seq]
     rcases cond with _ | _ <;> simp only
-    · rw [step_if_false x h₁ (by simp at eq; exact eq)]; rfl
-    · rw [step_if_true (by simp at eq; rw [eq] at h₁; exact h₁)]; rfl
+    · rw [run_if_false x h₁ (by simp at eq; exact eq)]; rfl
+    · rw [run_if_true (by simp at eq; rw [eq] at h₁; exact h₁)]; rfl
 
-lemma Cirgen.step_If_collapsible
+lemma Cirgen.run_If_collapsible
     {state : State}
     {name : String}
     {branch : Cirgen}
@@ -82,26 +82,26 @@ lemma Cirgen.step_If_collapsible
     Γ state ⟦guard ⟨name⟩ then branch⟧
   = if (x == 0)
       then (state, none)
-      else Cirgen.step state branch := by simp [step, h₁]
+      else Cirgen.run state branch := by simp [run, h₁]
 
-lemma Cirgen.step_Eqz_collapsible
+lemma Cirgen.run_Eqz_collapsible
     {state : State}
     {name : String}
     (x : Felt)
     (h₁ : state.felts name = some x) :
     Γ state ⟦?₀ ⟨name⟩⟧ 
-  = ({ state with constraints := x :: state.constraints }, none) := by simp [step, *]
+  = ({ state with constraints := x :: state.constraints }, none) := by simp [run, *]
 
-lemma Cirgen.step_Sequence_Eqz_collapsible
+lemma Cirgen.run_Sequence_Eqz_collapsible
     {state : State}
     {name : String}
     {program : Cirgen}
     (x : Felt)
     (h₁ : state.felts name = some x) :
-    Cirgen.step state (.Sequence (.Eqz (Variable.mk name)) program)
+    Cirgen.run state (.Sequence (.Eqz (Variable.mk name)) program)
   = let state₁ := { state with constraints := x :: state.constraints }
-    let (state₂, y) := Cirgen.step state₁ program
-    (state₂, y) := by rw [step_seq, step_Eqz_collapsible _ h₁]
+    let (state₂, y) := Cirgen.run state₁ program
+    (state₂, y) := by rw [run_seq, run_Eqz_collapsible _ h₁]
 
 end WithCirgen 
 
